@prefix : <http://linked.data.gov.au/def/placenames/> .
@prefix pt: <http://linked.data.gov.au/def/placetype/> .
@prefix geo: <http://www.opengis.net/ont/geosparql#> .
@prefix owl: <http://www.w3.org/2002/07/owl#> .
@prefix rdf: <http://www.w3.org/1999/02/22-rdf-syntax-ns#> .
@prefix reg: <http://purl.org/linked-data/registry#> .
@prefix xml: <http://www.w3.org/XML/1998/namespace> .
@prefix xsd: <http://www.w3.org/2001/XMLSchema#> .
@prefix loci: <http://linked.data.gov.au/def/loci#> .
@prefix prof: <http://www.w3.org/ns/dx/prof/> .
@prefix prov: <http://www.w3.org/ns/prov#> .
@prefix rdfs: <http://www.w3.org/2000/01/rdf-schema#> .
@prefix skos: <http://www.w3.org/2004/02/skos/core#> .
@prefix vann: <http://purl.org/vocab/vann/> .
@prefix schema: <https://schema.org/> .
@prefix dcterms: <http://purl.org/dc/terms/> .
@base <http://linked.data.gov.au/def/placenames> .

<http://linked.data.gov.au/def/placenames> rdf:type owl:Ontology ;
                                            owl:imports <http://www.opengis.net/ont/geosparql> ;
                                            dcterms:rights "(c) Commonwealth of Australia (Geoscience Australia) 2019, 2020" ;
                                            rdfs:comment """**Place Names** is an RDF/OWL Ontology to define the structure and relationship of the names of geospatial features, typically collected in a Gazetteer.

A place-name is a text string that

- is coined by an agent (person or organization)
- is authorized by a jurisidiction (national, state or local government) 
- is a member item in a gazetteer
- has lifecycle information (status, validity dates (TBD), formal identifier) 
- denotes a natural or constructed geospatial feature with a specified classification (inhabited place, administrative area, mountain, school, station, park ...)


This ontology uses classes and properties from existing vocabularies, in particular

- [GeoSPARQL](http://www.opengis.net/ont/geosparql)
- [SKOS](http://www.w3.org/2004/02/skos/core) 
- [Dublin Core](https://www.dublincore.org/specifications/dublin-core/dcmi-terms/)""" ;
                                            rdfs:label "Place Names Ontology"@en .

#################################################################
#    Annotation properties
#################################################################

###  http://purl.org/dc/terms/format
dcterms:format rdf:type owl:AnnotationProperty .


###  http://purl.org/dc/terms/identifier
dcterms:identifier rdf:type owl:AnnotationProperty .


###  http://purl.org/dc/terms/rights
dcterms:rights rdf:type owl:AnnotationProperty .


###  http://www.w3.org/2004/02/skos/core#altlabel
skos:altlabel rdf:type owl:AnnotationProperty .


###  https://schema.org/affiliation
schema:affiliation rdf:type owl:AnnotationProperty .


###  https://schema.org/email
schema:email rdf:type owl:AnnotationProperty .


###  https://schema.org/identifier
schema:identifier rdf:type owl:AnnotationProperty .


###  https://schema.org/memberOf
schema:memberOf rdf:type owl:AnnotationProperty .


###  https://schema.org/name
schema:name rdf:type owl:AnnotationProperty .


###  https://schema.org/uri
schema:uri rdf:type owl:AnnotationProperty .


#################################################################
#    Object Properties
#################################################################

###  http://linked.data.gov.au/def/loci#isMemberOf
loci:isMemberOf rdf:type owl:ObjectProperty .


###  http://linked.data.gov.au/def/placenames/hasPlaceClassification
:hasPlaceClassification rdf:type owl:ObjectProperty ;
                        rdfs:subPropertyOf dcterms:type ;
                        rdfs:domain :Place ;
                        rdfs:range :PlaceType ;
                        rdfs:comment "A relation between a Place and a classification of its real world phenomena."@en ;
                        rdfs:label "has place classification" .


###  http://linked.data.gov.au/def/placenames/hasPlaceName
:hasPlaceName rdf:type owl:ObjectProperty ;
              owl:inverseOf :placeNameOf ;
              rdfs:domain :Place ;
              rdfs:range :PlaceName ;
              rdfs:comment "The Feature has a place name (label) assigned to it"@en ;
              rdfs:label "has place name"@en ;
              skos:scopeNote "All PlaceName objects names indicated by hasPlaceName should have the role of the name indicated with a Name Type"@en .


###  http://linked.data.gov.au/def/placenames/hasPlaceNameFormality
:hasPlaceNameFormality rdf:type owl:ObjectProperty ;
                       rdfs:domain :PlaceName ;
                       rdfs:range :PlaceNameFormality ;
                       rdfs:comment "The formality of a Place Name"@en ;
                       rdfs:label "has place name formality"@en ;
                       skos:scopeNote "Values for this property must be selected from the Place Name Formality vocabulary"@en .


###  http://linked.data.gov.au/def/placenames/hasPlaceNamingAuthority
:hasPlaceNamingAuthority rdf:type owl:ObjectProperty ;
                         rdfs:subPropertyOf prov:wasAttributedTo ;
                         rdfs:domain :PlaceName ;
                         rdfs:range :Jurisdiction ;
                         rdfs:comment "The authority (jurisdiction) responsible for formally gazetting the place name."@en ;
                         rdfs:label "has place naming authority" .


###  http://linked.data.gov.au/def/placenames/placeNameOf
:placeNameOf rdf:type owl:ObjectProperty ;
             rdfs:domain :PlaceName ;
             rdfs:range :Place ;
             rdfs:label "place name of" .


###  http://linked.data.gov.au/def/placenames/status
:status rdf:type owl:ObjectProperty ;
        rdfs:domain :PlaceName ;
        rdfs:range :Status ;
        rdfs:label "has status" ;
        skos:scopeNote "This property indicates the status of a Place Name in a Gazetteer."@en .


###  http://linked.data.gov.au/def/placenames/wasNamedBy
:wasNamedBy rdf:type owl:ObjectProperty ;
            rdfs:subPropertyOf prov:wasAttributedTo ;
            rdfs:domain :PlaceName ;
            rdfs:range dcterms:Agent ;
            rdfs:comment "The Agent (person, community, organization) that assigned the name to the Place"@en ;
            rdfs:label "was named by"@en .


###  http://purl.org/dc/terms/contributor
dcterms:contributor rdf:type owl:ObjectProperty .


###  http://purl.org/dc/terms/creator
dcterms:creator rdf:type owl:ObjectProperty .


###  http://purl.org/dc/terms/publisher
dcterms:publisher rdf:type owl:ObjectProperty .


###  http://purl.org/dc/terms/type
dcterms:type rdf:type owl:ObjectProperty .


###  http://www.w3.org/2000/01/rdf-schema#member
rdfs:member rdf:type owl:ObjectProperty .


###  http://www.w3.org/2004/02/skos/core#broader
skos:broader rdf:type owl:ObjectProperty .


###  http://www.w3.org/2004/02/skos/core#exactMatch
skos:exactMatch rdf:type owl:ObjectProperty .


###  http://www.w3.org/2004/02/skos/core#inScheme
skos:inScheme rdf:type owl:ObjectProperty .


###  http://www.w3.org/2004/02/skos/core#topConceptOf
skos:topConceptOf rdf:type owl:ObjectProperty .


###  http://www.w3.org/ns/dx/prof/hasArtifact
prof:hasArtifact rdf:type owl:ObjectProperty .


###  http://www.w3.org/ns/dx/prof/hasResource
prof:hasResource rdf:type owl:ObjectProperty .


###  http://www.w3.org/ns/dx/prof/hasRole
prof:hasRole rdf:type owl:ObjectProperty .


###  http://www.w3.org/ns/dx/prof/isProfileOf
prof:isProfileOf rdf:type owl:ObjectProperty .


###  http://www.w3.org/ns/prov#wasAttributedTo
prov:wasAttributedTo rdf:type owl:ObjectProperty .


#################################################################
#    Data properties
#################################################################

###  http://linked.data.gov.au/def/placenames/hasPronunciation
:hasPronunciation rdf:type owl:DatatypeProperty ;
                  rdfs:domain :PlaceName ;
                  rdfs:range xsd:string ;
                  rdfs:comment "The pronunciation of a Place Name, indicated by means of a phonetic alphabet string"@en ;
                  rdfs:label "pronunciation"@en .


###  http://linked.data.gov.au/def/placenames/name
:name rdf:type owl:DatatypeProperty ;
      rdfs:domain :PlaceName ;
      rdfs:range xsd:string ;
      rdfs:label "name" .


###  http://purl.org/dc/terms/created
dcterms:created rdf:type owl:DatatypeProperty .


###  http://purl.org/dc/terms/identifier
dcterms:identifier rdf:type owl:DatatypeProperty .


###  http://purl.org/dc/terms/modified
dcterms:modified rdf:type owl:DatatypeProperty .


#################################################################
#    Classes
#################################################################

###  http://linked.data.gov.au/def/loci#Dataset
loci:Dataset rdf:type owl:Class .


###  http://linked.data.gov.au/def/placenames/Gazetteer
:Gazetteer rdf:type owl:Class ;
           rdfs:subClassOf loci:Dataset ,
                           rdf:Bag ,
                           [ rdf:type owl:Restriction ;
                             owl:onProperty rdfs:member ;
                             owl:allValuesFrom :PlaceName
                           ] ;
           rdfs:comment "A Gazetteer is a list of Place Names"@en ;
           rdfs:label "Gazetteer"@en ;
           skos:changeNote """
was- 
```
  	rdfs:subClassOf reg:Register ;
  	rdfs:subClassOf [
      rdf:type owl:Restriction ;
      owl:hasValue :PlaceName ;
      owl:onProperty reg:containedItemClass ;
    ] ;
```
But this is not appropriate - according to the Registry Ontology a reg:Register is a set of metadata records, not a set of Entities. 

Use `rdf:Bag` and `rdfs:member` instead. 
""" .


###  http://linked.data.gov.au/def/placenames/Jurisdiction
:Jurisdiction rdf:type owl:Class ;
              rdfs:subClassOf dcterms:Agent ;
              rdfs:comment "Local, State, Territory or National (Commonwealth) Government that has authority to formally establish (i.e. gazette) place names within its jurisdictional area."@en ;
              rdfs:label "Jurisdiction" .


###  http://linked.data.gov.au/def/placenames/Place
:Place rdf:type owl:Class ;
       rdfs:subClassOf geo:Feature ,
                       [ rdf:type owl:Restriction ;
                         owl:onProperty loci:isMemberOf ;
                         owl:someValuesFrom :Gazetteer
                       ] ,
                       [ rdf:type owl:Restriction ;
                         owl:onProperty :hasPlaceClassification ;
                         owl:minCardinality "1"^^xsd:nonNegativeInteger
                       ] ,
                       [ rdf:type owl:Restriction ;
                         owl:onProperty geo:hasGeometry ;
                         owl:minQualifiedCardinality "1"^^xsd:nonNegativeInteger ;
                         owl:onClass geo:Geometry
                       ] ,
                       [ rdf:type owl:Restriction ;
                         owl:onProperty dcterms:identifier ;
                         owl:minCardinality "1"^^xsd:nonNegativeInteger
                       ] ;
       rdfs:comment "An identifiable geographic Place as defined by the Composite Gazetteer of Australia. A Place is classified according to an extensible set of types."@en ;
       rdfs:label "Place"@en .


###  http://linked.data.gov.au/def/placenames/PlaceName
:PlaceName rdf:type owl:Class ;
           rdfs:subClassOf [ rdf:type owl:Restriction ;
                             owl:onProperty loci:isMemberOf ;
                             owl:someValuesFrom :Gazetteer
                           ] ,
                           [ rdf:type owl:Restriction ;
                             owl:onProperty :placeNameOf ;
                             owl:minCardinality "1"^^xsd:nonNegativeInteger
                           ] ,
                           [ rdf:type owl:Restriction ;
                             owl:onProperty :hasPlaceNamingAuthority ;
                             owl:cardinality "1"^^xsd:nonNegativeInteger
                           ] ,
                           [ rdf:type owl:Restriction ;
                             owl:onProperty :status ;
                             owl:cardinality "1"^^xsd:nonNegativeInteger
                           ] ,
                           [ rdf:type owl:Restriction ;
                             owl:onProperty dcterms:identifier ;
                             owl:minCardinality "1"^^xsd:nonNegativeInteger
                           ] ,
                           [ rdf:type owl:Restriction ;
                             owl:onProperty :name ;
                             owl:cardinality "1"^^xsd:nonNegativeInteger
                           ] ;
           rdfs:comment "The name of a place, assigned by an official naming authority and included in the Place Names Gazeteer of Australia."@en ;
           rdfs:label "Place Name"@en ;
           skos:changeNote "Removed subClassOf reg:RegisterItem axiom, because reg:RegisterItem is \"A metadata record for an entry in a register. \" and is not an Entity itself. " .


###  http://linked.data.gov.au/def/placenames/PlaceNameFormality
:PlaceNameFormality rdf:type owl:Class ;
                    rdfs:subClassOf skos:Concept ;
                    rdfs:comment "The formality of a Place Name: official, historical, informal"@en ;
                    rdfs:label "Place Name Formality"@en .


###  http://linked.data.gov.au/def/placenames/PlaceType
:PlaceType rdf:type owl:Class ;
           rdfs:subClassOf skos:Concept ;
           rdfs:comment "The classification of a place, from the ICSM Permanent Committee on Place Names classification scheme."@en ;
           rdfs:label "Place Type"@en .


###  http://linked.data.gov.au/def/placenames/PointOfInterest
:PointOfInterest rdf:type owl:Class ;
                 rdfs:subClassOf :Place ,
                                 [ rdf:type owl:Restriction ;
                                   owl:onProperty :hasPlaceClassification ;
                                   owl:hasValue pt:PointOfInterest
                                 ] ;
                 rdfs:comment "A specific point Location that someone may find useful or interesting."@en ;
                 rdfs:label "Point of Interest"@en .


###  http://linked.data.gov.au/def/placenames/Region
:Region rdf:type owl:Class ;
        rdfs:subClassOf :Place ,
                        [ rdf:type owl:Restriction ;
                          owl:onProperty :hasPlaceClassification ;
                          owl:hasValue pt:Region
                        ] ;
        rdfs:comment "A Region is an area of land that has common features."@en ;
        rdfs:label "Region"@en .


###  http://linked.data.gov.au/def/placenames/Status
:Status rdf:type owl:Class ;
        rdfs:subClassOf skos:Concept ;
        rdfs:label "Status " .


###  http://purl.org/dc/terms/Agent
dcterms:Agent rdf:type owl:Class .


###  http://www.w3.org/1999/02/22-rdf-syntax-ns#Bag
rdf:Bag rdf:type owl:Class .


###  https://schema.org/Person
schema:Person rdf:type owl:Class .


#################################################################
#    Individuals
#################################################################

###  http://linked.data.gov.au/def/placenames
<http://linked.data.gov.au/def/placenames> rdf:type owl:NamedIndividual ;
                                           dcterms:contributor <https://orcid.org/0000-0002-4643-7289> ,
                                                               <https://orcid.org/0000-0003-3425-0780> ;
                                           dcterms:creator <https://orcid.org/0000-0002-3884-3420> ,
                                                           <https://orcid.org/0000-0002-8742-7730> ;
                                           dcterms:publisher [ rdfs:seeAlso <https://www.ga.gov.au> ;
                                                               schema:identifier "http://catalogue.linked.data.gov.au/org/ga" ;
                                                               schema:name "Geoscience Australia"
                                                             ] ;
                                           prof:hasResource _:genid15 ,
                                                            _:genid16 ;
                                           prof:isProfileOf <http://www.opengis.net/doc/IS/geosparql/1.0> ;
                                           dcterms:created "2018-08-02"^^xsd:date ;
                                           dcterms:modified "2020-02-19"^^xsd:date .

_:genid15 prof:hasArtifact <http://linked.data.gov.au/def/placenames> ;
           prof:hasRole <http://www.w3.org/ns/dx/prof/role/specification> ;
           dcterms:format <https://w3id.org/mediatype/text/html> .

_:genid16 prof:hasArtifact <http://linked.data.gov.au/def/placenames.ttl> ;
           prof:hasRole <http://www.w3.org/ns/dx/prof/role/schema> ;
           dcterms:format <https://w3id.org/mediatype/text/turtle> .


###  http://linked.data.gov.au/def/placenames.ttl
<http://linked.data.gov.au/def/placenames.ttl> rdf:type owl:NamedIndividual .


###  http://linked.data.gov.au/def/placenames/Historical
:Historical rdf:type owl:NamedIndividual ,
                     :PlaceNameFormality ;
            rdfs:label "Historical" ;
            skos:prefLabel "Historical" .


###  http://linked.data.gov.au/def/placenames/Informal
:Informal rdf:type owl:NamedIndividual ,
                   :PlaceNameFormality ;
          rdfs:label "Informal" ;
          skos:prefLabel "Informal" .


###  http://linked.data.gov.au/def/placenames/Official
:Official rdf:type owl:NamedIndividual ,
                   :PlaceNameFormality ;
          rdfs:label "Official" ;
          skos:prefLabel "Official" .


###  http://linked.data.gov.au/def/placenames/StatusScheme
:StatusScheme rdf:type owl:NamedIndividual ,
                       skos:ConceptScheme .


###  http://linked.data.gov.au/def/placenames/statusAccepted
:statusAccepted rdf:type owl:NamedIndividual ,
                         :Status ;
                skos:exactMatch reg:statusAccepted ;
                skos:topConceptOf :StatusScheme ;
                rdfs:comment "An entry that has been accepted for use and is visible in the default register listing. Includes entries that have seen been retired or superseded."@en ;
                skos:definition "An entry that has been accepted for use and is visible in the default register listing. Includes entries that have seen been retired or superseded."@en ;
                skos:prefLabel "accepted"@en .


###  http://linked.data.gov.au/def/placenames/statusDeprecated
:statusDeprecated rdf:type owl:NamedIndividual ,
                           :Status ;
                  skos:broader :statusAccepted ;
                  skos:exactMatch reg:statusDeprecated ;
                  skos:inScheme :StatusScheme ;
                  rdfs:comment "An entry that has been retired or replaced and is no longer to be used."@en ;
                  skos:definition "An entry that has been retired or replaced and is no longer to be used."@en ;
                  skos:prefLabel "deprecated"@en .


###  http://linked.data.gov.au/def/placenames/statusExperimental
:statusExperimental rdf:type owl:NamedIndividual ,
                             :Status ;
                    skos:broader :statusValid ;
                    skos:exactMatch reg:statusExperimental ;
                    skos:inScheme :StatusScheme ;
                    rdfs:comment "An entry that has been accepted into the register temporarily and may be subject to change or withdrawal."@en ;
                    skos:altlabel "provisional"@en ;
                    skos:definition "An entry that has been accepted into the register temporarily and may be subject to change or withdrawal."@en ;
                    skos:prefLabel "experimental"@en .


###  http://linked.data.gov.au/def/placenames/statusInvalid
:statusInvalid rdf:type owl:NamedIndividual ,
                        :Status ;
               skos:broader :statusNotAccepted ;
               skos:exactMatch reg:statusInvalid ;
               skos:inScheme :StatusScheme ;
               rdfs:comment "An entry which has been invalidated due to serious flaws, distinct from retrirement. Corresponds to ISO 19135(redraft) 'invalid'"@en ;
               skos:definition "An entry which has been invalidated due to serious flaws, distinct from retrirement. Corresponds to ISO 19135(redraft) 'invalid'"@en ;
               skos:prefLabel "invalid"@en .


###  http://linked.data.gov.au/def/placenames/statusNotAccepted
:statusNotAccepted rdf:type owl:NamedIndividual ,
                            :Status ;
                   skos:exactMatch reg:statusNotAccepted ;
                   skos:topConceptOf :StatusScheme ;
                   rdfs:comment "An entry that should not be visible in the default register listing. Corresponds to ISO 19135:2005 'notValid'"@en ;
                   skos:definition "An entry that should not be visible in the default register listing. Corresponds to ISO 19135:2005 'notValid'"@en ;
                   skos:prefLabel "notAccepted"@en .


###  http://linked.data.gov.au/def/placenames/statusReserved
:statusReserved rdf:type owl:NamedIndividual ,
                         :Status ;
                skos:broader :statusNotAccepted ;
                skos:exactMatch reg:statusReserved ;
                skos:inScheme :StatusScheme ;
                rdfs:comment "A reserved entry allocated for some as yet undetermined future use."@en ;
                skos:definition "A reserved entry allocated for some as yet undetermined future use."@en ;
                skos:prefLabel "reserved"@en .


###  http://linked.data.gov.au/def/placenames/statusRetired
:statusRetired rdf:type owl:NamedIndividual ,
                        :Status ;
               skos:broader :statusDeprecated ;
               skos:exactMatch reg:statusRetired ;
               rdfs:comment "An entry that has been withdrawn from use.  Corresponds to ISO 19135:2005 'retired'"@en ;
               skos:altlabel "withdrawn"@en ;
               skos:definition "An entry that has been withdrawn from use.  Corresponds to ISO 19135:2005 'retired'"@en ;
               skos:prefLabel "retired"@en .


###  http://linked.data.gov.au/def/placenames/statusStable
:statusStable rdf:type owl:NamedIndividual ,
                       :Status ;
              skos:broader :statusValid ;
              skos:exactMatch reg:statusStable ;
              skos:inScheme :StatusScheme ;
              rdfs:comment "An entry that is seen as having a reasonable measure of stability, may be used to mark the full adoption of a previously 'experimental' entry."@en ;
              skos:definition "An entry that is seen as having a reasonable measure of stability, may be used to mark the full adoption of a previously 'experimental' entry."@en ;
              skos:prefLabel "stable"@en .


###  http://linked.data.gov.au/def/placenames/statusSubmitted
:statusSubmitted rdf:type owl:NamedIndividual ,
                          :Status ;
                 skos:broader :statusNotAccepted ;
                 skos:exactMatch reg:statusSubmitted ;
                 skos:inScheme :StatusScheme ;
                 rdfs:comment "A proposed entry which is not yet approved for use for use. Corresponds to ISO 19135:(redraft) 'submitted'"@en ;
                 skos:definition "A proposed entry which is not yet approved for use for use. Corresponds to ISO 19135:(redraft) 'submitted'"@en ;
                 skos:prefLabel "submitted"@en .


###  http://linked.data.gov.au/def/placenames/statusSuperseded
:statusSuperseded rdf:type owl:NamedIndividual ,
                           :Status ;
                  skos:broader :statusDeprecated ;
                  skos:exactMatch reg:statusSuperseded ;
                  skos:inScheme :StatusScheme ;
                  rdfs:comment "An entry that has been replaced by a new alternative which should be used instead.  Corresponds to ISO 19135:2005 'superseded'."@en ;
                  skos:altlabel "replaced"@en ;
                  skos:definition "An entry that has been replaced by a new alternative which should be used instead.  Corresponds to ISO 19135:2005 'superseded'."@en ;
                  skos:prefLabel "superseded"@en .


###  http://linked.data.gov.au/def/placenames/statusValid
:statusValid rdf:type owl:NamedIndividual ,
                      :Status ;
             skos:broader :statusAccepted ;
             skos:exactMatch reg:statusValid ;
             skos:inScheme :StatusScheme ;
             rdfs:comment "An entry that has been accepted into the register and is deemed fit for use. Corresponds to ISO 19135:2005 'valid'."@en ;
             skos:definition "An entry that has been accepted into the register and is deemed fit for use. Corresponds to ISO 19135:2005 'valid'."@en ;
             skos:prefLabel "valid"@en .


###  http://linked.data.gov.au/def/placetype/PointOfInterest
pt:PointOfInterest rdf:type owl:NamedIndividual ,
                            :PlaceType ;
                   rdfs:label "Point of interest" .


###  http://linked.data.gov.au/def/placetype/Region
pt:Region rdf:type owl:NamedIndividual ,
                   :PlaceType ;
          rdfs:label "Region" .


###  http://purl.org/linked-data/registry#statusAccepted
reg:statusAccepted rdf:type owl:NamedIndividual .


###  http://purl.org/linked-data/registry#statusDeprecated
reg:statusDeprecated rdf:type owl:NamedIndividual .


###  http://purl.org/linked-data/registry#statusExperimental
reg:statusExperimental rdf:type owl:NamedIndividual .


###  http://purl.org/linked-data/registry#statusInvalid
reg:statusInvalid rdf:type owl:NamedIndividual .


###  http://purl.org/linked-data/registry#statusNotAccepted
reg:statusNotAccepted rdf:type owl:NamedIndividual .


###  http://purl.org/linked-data/registry#statusReserved
reg:statusReserved rdf:type owl:NamedIndividual .


###  http://purl.org/linked-data/registry#statusRetired
reg:statusRetired rdf:type owl:NamedIndividual .


###  http://purl.org/linked-data/registry#statusStable
reg:statusStable rdf:type owl:NamedIndividual .


###  http://purl.org/linked-data/registry#statusSubmitted
reg:statusSubmitted rdf:type owl:NamedIndividual .


###  http://purl.org/linked-data/registry#statusSuperseded
reg:statusSuperseded rdf:type owl:NamedIndividual .


###  http://purl.org/linked-data/registry#statusValid
reg:statusValid rdf:type owl:NamedIndividual .


###  http://www.opengis.net/doc/IS/geosparql/1.0
<http://www.opengis.net/doc/IS/geosparql/1.0> rdf:type owl:NamedIndividual .


###  http://www.w3.org/ns/dx/prof/role/schema
<http://www.w3.org/ns/dx/prof/role/schema> rdf:type owl:NamedIndividual .


###  http://www.w3.org/ns/dx/prof/role/specification
<http://www.w3.org/ns/dx/prof/role/specification> rdf:type owl:NamedIndividual .


###  https://orcid.org/0000-0002-3884-3420
<https://orcid.org/0000-0002-3884-3420> rdf:type owl:NamedIndividual ,
                                                 schema:Person ;
                                        schema:affiliation [ schema:identifier "http://catalogue.linked.data.gov.au/org/csiro"^^xsd:anyURI ;
                                                             schema:name "CSIRO"
                                                           ] ;
                                        schema:email <mailto:simon.cox@csiro.au> ;
                                        schema:identifier "https://orcid.org/0000-0002-3884-3420"^^xsd:anyURI ;
                                        schema:name "Simon J D Cox"@en .


###  https://orcid.org/0000-0002-4643-7289
<https://orcid.org/0000-0002-4643-7289> rdf:type owl:NamedIndividual ,
                                                 schema:Person ;
                                        schema:affiliation [ schema:identifier "http://catalogue.linked.data.gov.au/org/ga"^^xsd:anyURI ;
                                                             schema:name "Geoscience Australia"
                                                           ] ;
                                        schema:email <mailto:irina.bastrakova@ga.gov.au> ;
                                        schema:identifier "https://orcid.org/0000-0002-4643-7289"^^xsd:anyURI ;
                                        schema:name "Irina Bastrakova"@en .


###  https://orcid.org/0000-0002-8742-7730
<https://orcid.org/0000-0002-8742-7730> rdf:type owl:NamedIndividual ,
                                                 schema:Person ;
                                        schema:affiliation [ schema:name "Surround Australia" ;
                                                             schema:uri <https://surroundaustralia.com/>
                                                           ] ;
                                        schema:email <mailto:nicholas.car@surroundaustralia.com> ;
                                        schema:identifier "https://orcid.org/0000-0002-8742-7730"^^xsd:anyURI ;
                                        schema:name "Nicholas Car"@en .


###  https://orcid.org/0000-0003-3425-0780
<https://orcid.org/0000-0003-3425-0780> rdf:type owl:NamedIndividual ,
                                                 schema:Person ;
                                        schema:affiliation [ schema:identifier "http://catalogue.linked.data.gov.au/org/anu"^^xsd:anyURI ;
                                                             schema:name "Australian National University"
                                                           ] ,
                                                           [ schema:identifier "http://catalogue.linked.data.gov.au/org/anu"^^xsd:anyURI ;
                                                             schema:name "Australian National University"
                                                           ] ;
                                        schema:email <mailto:armin.haller@anu.edu.au> ;
                                        schema:identifier "https://orcid.org/0000-0003-3425-0780"^^xsd:anyURI ;
                                        schema:name "Armin Haller"@en .


_:genid22 prof:hasArtifact <http://linked.data.gov.au/def/placenames.ttl> ;
          prof:hasRole <http://www.w3.org/ns/dx/prof/role/schema> ;
          dcterms:format <https://w3id.org/mediatype/text/turtle> .

_:genid23 prof:hasArtifact <http://linked.data.gov.au/def/placenames> ;
           prof:hasRole <http://www.w3.org/ns/dx/prof/role/specification> ;
           dcterms:format <https://w3id.org/mediatype/text/html> .

###  Generated by the OWL API (version 4.5.9.2019-02-01T07:24:44Z) https://github.com/owlcs/owlapi
