# baseURI: http://linked.data.gov.au/def/placenames
# imports: http://www.opengis.net/ont/geosparql

@prefix : <http://linked.data.gov.au/def/placenames/> .
@prefix dcterms: <http://purl.org/dc/terms/> .
@prefix geo: <http://www.opengis.net/ont/geosparql#> .
@prefix loci: <http://linked.data.gov.au/def/loci#> .
@prefix owl: <http://www.w3.org/2002/07/owl#> .
@prefix prof: <http://www.w3.org/ns/dx/prof/> .
@prefix prov: <http://www.w3.org/ns/prov#> .
@prefix pt: <http://linked.data.gov.au/def/placetype/> .
@prefix rdf: <http://www.w3.org/1999/02/22-rdf-syntax-ns#> .
@prefix rdfs: <http://www.w3.org/2000/01/rdf-schema#> .
@prefix reg: <http://purl.org/linked-data/registry#> .
@prefix schema: <https://schema.org/> .
@prefix skos: <http://www.w3.org/2004/02/skos/core#> .
@prefix vann: <http://purl.org/vocab/vann/> .
@prefix xml: <http://www.w3.org/XML/1998/namespace> .
@prefix xsd: <http://www.w3.org/2001/XMLSchema#> .

loci:Dataset
  a owl:Class ;
.
loci:isMemberOf
  a owl:ObjectProperty ;
.
<http://linked.data.gov.au/def/placenames>
  a owl:NamedIndividual ;
  a owl:Ontology ;
  dcterms:contributor <https://orcid.org/0000-0002-4643-7289> ;
  dcterms:contributor <https://orcid.org/0000-0003-3425-0780> ;
  dcterms:created "2018-08-02"^^xsd:date ;
  dcterms:creator <https://orcid.org/0000-0002-3884-3420> ;
  dcterms:creator <https://orcid.org/0000-0002-8742-7730> ;
  dcterms:modified "2020-05-21"^^xsd:date ;
  dcterms:publisher [
      rdfs:seeAlso <https://www.ga.gov.au> ;
      schema:identifier "http://catalogue.linked.data.gov.au/org/ga" ;
      schema:name "Geoscience Australia" ;
    ] ;
  dcterms:rights "(c) Commonwealth of Australia (Geoscience Australia) 2019, 2020" ;
  dcterms:title "Place Names Ontology"@en ;
  rdfs:comment """**Place Names** is an RDF/OWL Ontology to define the structure and relationship of the names of geospatial features, typically collected in a Gazetteer.

A place-name is a text string that

- is coined by an agent (person or organization)
- is authorized by a jurisidiction (national, state or local government) 
- is a member item in a gazetteer
- has lifecycle information (status, validity dates (TBD), formal identifier) 
- denotes a natural or constructed geospatial feature with a specified classification (inhabited place, administrative area, mountain, school, station, park ...)

This ontology uses classes and properties from existing vocabularies, in particular

- [GeoSPARQL](http://www.opengis.net/ont/geosparql)
- [SKOS](http://www.w3.org/2004/02/skos/core) 
- [Dublin Core](https://www.dublincore.org/specifications/dublin-core/dcmi-terms/)

![](./images/placename-details.png)""" ;
  rdfs:label "Place Names Ontology"@en ;
  owl:imports <http://www.opengis.net/ont/geosparql> ;
  prof:hasResource [
      dcterms:format <https://w3id.org/mediatype/text/html> ;
      prof:hasArtifact <http://linked.data.gov.au/def/placenames> ;
      prof:hasRole <http://www.w3.org/ns/dx/prof/role/specification> ;
    ] ;
  prof:hasResource [
      dcterms:format <https://w3id.org/mediatype/text/turtle> ;
      prof:hasArtifact <http://linked.data.gov.au/def/placenames.ttl> ;
      prof:hasRole <http://www.w3.org/ns/dx/prof/role/schema> ;
    ] ;
  prof:isProfileOf <http://www.opengis.net/doc/IS/geosparql/1.0> ;
.
<http://linked.data.gov.au/def/placenames.ttl>
  a owl:NamedIndividual ;
.
:Gazetteer
  a owl:Class ;
  rdfs:comment "A Gazetteer is a list of Place Names"@en ;
  rdfs:label "Gazetteer"@en ;
  rdfs:subClassOf loci:Dataset ;
  rdfs:subClassOf rdf:Bag ;
  rdfs:subClassOf [
      a owl:Restriction ;
      owl:allValuesFrom :PlaceName ;
      owl:onProperty rdfs:member ;
    ] ;
  skos:changeNote """
was- 
```
  	rdfs:subClassOf reg:Register ;
  	rdfs:subClassOf [
      rdf:type owl:Restriction ;
      owl:hasValue :PlaceName ;
      owl:onProperty reg:containedItemClass ;
    ] ;
```
But this is not appropriate - according to the Registry Ontology a reg:Register is a set of metadata records, not a set of Entities. 

Use `rdf:Bag` and `rdfs:member` instead. 
""" ;
.
:Historical
  a :PlaceNameFormality ;
  a owl:NamedIndividual ;
  rdfs:label "Historical" ;
  skos:prefLabel "Historical" ;
.
:Informal
  a :PlaceNameFormality ;
  a owl:NamedIndividual ;
  rdfs:label "Informal" ;
  skos:prefLabel "Informal" ;
.
:Jurisdiction
  a owl:Class ;
  rdfs:comment "Local, State, Territory or National (Commonwealth) Government that has authority to formally establish (i.e. gazette) place names within its jurisdictional area."@en ;
  rdfs:label "Jurisdiction" ;
  rdfs:subClassOf dcterms:Agent ;
.
:Official
  a :PlaceNameFormality ;
  a owl:NamedIndividual ;
  rdfs:label "Official" ;
  skos:prefLabel "Official" ;
.
:Place
  a owl:Class ;
  rdfs:comment "An identifiable geographic Place as defined by the Composite Gazetteer of Australia. A Place is classified according to an extensible set of types."@en ;
  rdfs:label "Place"@en ;
  rdfs:subClassOf geo:Feature ;
  rdfs:subClassOf [
      a owl:Restriction ;
      owl:minCardinality "1"^^xsd:nonNegativeInteger ;
      owl:onProperty :hasPlaceClassification ;
    ] ;
  rdfs:subClassOf [
      a owl:Restriction ;
      owl:minCardinality "1"^^xsd:nonNegativeInteger ;
      owl:onProperty dcterms:identifier ;
    ] ;
  rdfs:subClassOf [
      a owl:Restriction ;
      owl:minQualifiedCardinality "1"^^xsd:nonNegativeInteger ;
      owl:onClass geo:Geometry ;
      owl:onProperty geo:hasGeometry ;
    ] ;
.
:PlaceName
  a owl:Class ;
  rdfs:comment "The name of a place, assigned by an official naming authority and included in the Place Names Gazeteer of Australia."@en ;
  rdfs:label "Place Name"@en ;
  rdfs:subClassOf [
      a owl:Restriction ;
      owl:cardinality "1"^^xsd:nonNegativeInteger ;
      owl:onProperty :hasPlaceNamingAuthority ;
    ] ;
  rdfs:subClassOf [
      a owl:Restriction ;
      owl:cardinality "1"^^xsd:nonNegativeInteger ;
      owl:onProperty :name ;
    ] ;
  rdfs:subClassOf [
      a owl:Restriction ;
      owl:cardinality "1"^^xsd:nonNegativeInteger ;
      owl:onProperty :status ;
    ] ;
  rdfs:subClassOf [
      a owl:Restriction ;
      owl:minCardinality "1"^^xsd:nonNegativeInteger ;
      owl:onProperty :placeNameOf ;
    ] ;
  rdfs:subClassOf [
      a owl:Restriction ;
      owl:minCardinality "1"^^xsd:nonNegativeInteger ;
      owl:onProperty dcterms:identifier ;
    ] ;
  rdfs:subClassOf [
      a owl:Restriction ;
      owl:onProperty loci:isMemberOf ;
      owl:someValuesFrom :Gazetteer ;
    ] ;
  skos:changeNote "Removed subClassOf reg:RegisterItem axiom, because reg:RegisterItem is \"A metadata record for an entry in a register. \" and is not an Entity itself. " ;
.
:PlaceNameFormality
  a owl:Class ;
  rdfs:comment "The formality of a Place Name: official, historical, informal"@en ;
  rdfs:label "Place Name Formality"@en ;
  rdfs:subClassOf skos:Concept ;
.
:PlaceType
  a owl:Class ;
  rdfs:comment "The classification of a place, from the ICSM Permanent Committee on Place Names classification scheme."@en ;
  rdfs:label "Place Type"@en ;
  rdfs:subClassOf skos:Concept ;
.
:PointOfInterest
  a owl:Class ;
  rdfs:comment "A specific point Location that someone may find useful or interesting."@en ;
  rdfs:label "Point of Interest"@en ;
  rdfs:subClassOf :Place ;
  rdfs:subClassOf [
      a owl:Restriction ;
      owl:hasValue pt:PointOfInterest ;
      owl:onProperty :hasPlaceClassification ;
    ] ;
.
:Region
  a owl:Class ;
  rdfs:comment "A Region is an area of land that has common features."@en ;
  rdfs:label "Region"@en ;
  rdfs:subClassOf :Place ;
  rdfs:subClassOf [
      a owl:Restriction ;
      owl:hasValue pt:Region ;
      owl:onProperty :hasPlaceClassification ;
    ] ;
.
:Status
  a owl:Class ;
  rdfs:label "Status " ;
  rdfs:subClassOf skos:Concept ;
.
:StatusScheme
  a owl:NamedIndividual ;
  a skos:ConceptScheme ;
.
:hasPlaceClassification
  a owl:ObjectProperty ;
  rdfs:comment "A relation between a Place and a classification of its real world phenomena."@en ;
  rdfs:domain :Place ;
  rdfs:label "has place classification" ;
  rdfs:range :PlaceType ;
  rdfs:subPropertyOf dcterms:type ;
.
:hasPlaceName
  a owl:ObjectProperty ;
  rdfs:comment "The Feature has a place name (label) assigned to it"@en ;
  rdfs:domain :Place ;
  rdfs:label "has place name"@en ;
  rdfs:range :PlaceName ;
  owl:inverseOf :placeNameOf ;
  skos:scopeNote "All PlaceName objects names indicated by hasPlaceName should have the role of the name indicated with a Name Type"@en ;
.
:hasPlaceNameFormality
  a owl:ObjectProperty ;
  rdfs:comment "The formality of a Place Name"@en ;
  rdfs:domain :PlaceName ;
  rdfs:label "has place name formality"@en ;
  rdfs:range :PlaceNameFormality ;
  skos:scopeNote "Values for this property must be selected from the Place Name Formality vocabulary"@en ;
.
:hasPlaceNamingAuthority
  a owl:ObjectProperty ;
  rdfs:comment "The authority (jurisdiction) responsible for formally gazetting the place name."@en ;
  rdfs:domain :PlaceName ;
  rdfs:label "has place naming authority" ;
  rdfs:range :Jurisdiction ;
  rdfs:subPropertyOf prov:wasAttributedTo ;
.
:hasPronunciation
  a owl:DatatypeProperty ;
  rdfs:comment "The pronunciation of a Place Name, indicated by means of a phonetic alphabet string"@en ;
  rdfs:domain :PlaceName ;
  rdfs:label "pronunciation"@en ;
  rdfs:range xsd:string ;
.
:isIndigenous
  a owl:DatatypeProperty ;
  rdfs:domain :PlaceName ;
  rdfs:label "name is indigenous" ;
  rdfs:range xsd:boolean ;
.
:name
  a owl:DatatypeProperty ;
  rdfs:domain :PlaceName ;
  rdfs:label "name" ;
  rdfs:range xsd:string ;
.
:placeNameOf
  a owl:ObjectProperty ;
  rdfs:domain :PlaceName ;
  rdfs:label "place name of" ;
  rdfs:range :Place ;
.
:status
  a owl:ObjectProperty ;
  rdfs:domain :PlaceName ;
  rdfs:label "has status" ;
  rdfs:range :Status ;
  skos:scopeNote "This property indicates the status of a Place Name in a Gazetteer."@en ;
.
:statusAccepted
  a :Status ;
  a owl:NamedIndividual ;
  rdfs:comment "An entry that has been accepted for use and is visible in the default register listing. Includes entries that have seen been retired or superseded."@en ;
  skos:definition "An entry that has been accepted for use and is visible in the default register listing. Includes entries that have seen been retired or superseded."@en ;
  skos:exactMatch reg:statusAccepted ;
  skos:prefLabel "accepted"@en ;
  skos:topConceptOf :StatusScheme ;
.
:statusDeprecated
  a :Status ;
  a owl:NamedIndividual ;
  rdfs:comment "An entry that has been retired or replaced and is no longer to be used."@en ;
  skos:broader :statusAccepted ;
  skos:definition "An entry that has been retired or replaced and is no longer to be used."@en ;
  skos:exactMatch reg:statusDeprecated ;
  skos:inScheme :StatusScheme ;
  skos:prefLabel "deprecated"@en ;
.
:statusExperimental
  a :Status ;
  a owl:NamedIndividual ;
  rdfs:comment "An entry that has been accepted into the register temporarily and may be subject to change or withdrawal."@en ;
  skos:altlabel "provisional"@en ;
  skos:broader :statusValid ;
  skos:definition "An entry that has been accepted into the register temporarily and may be subject to change or withdrawal."@en ;
  skos:exactMatch reg:statusExperimental ;
  skos:inScheme :StatusScheme ;
  skos:prefLabel "experimental"@en ;
.
:statusInvalid
  a :Status ;
  a owl:NamedIndividual ;
  rdfs:comment "An entry which has been invalidated due to serious flaws, distinct from retrirement. Corresponds to ISO 19135(redraft) 'invalid'"@en ;
  skos:broader :statusNotAccepted ;
  skos:definition "An entry which has been invalidated due to serious flaws, distinct from retrirement. Corresponds to ISO 19135(redraft) 'invalid'"@en ;
  skos:exactMatch reg:statusInvalid ;
  skos:inScheme :StatusScheme ;
  skos:prefLabel "invalid"@en ;
.
:statusNotAccepted
  a :Status ;
  a owl:NamedIndividual ;
  rdfs:comment "An entry that should not be visible in the default register listing. Corresponds to ISO 19135:2005 'notValid'"@en ;
  skos:definition "An entry that should not be visible in the default register listing. Corresponds to ISO 19135:2005 'notValid'"@en ;
  skos:exactMatch reg:statusNotAccepted ;
  skos:prefLabel "notAccepted"@en ;
  skos:topConceptOf :StatusScheme ;
.
:statusReserved
  a :Status ;
  a owl:NamedIndividual ;
  rdfs:comment "A reserved entry allocated for some as yet undetermined future use."@en ;
  skos:broader :statusNotAccepted ;
  skos:definition "A reserved entry allocated for some as yet undetermined future use."@en ;
  skos:exactMatch reg:statusReserved ;
  skos:inScheme :StatusScheme ;
  skos:prefLabel "reserved"@en ;
.
:statusRetired
  a :Status ;
  a owl:NamedIndividual ;
  rdfs:comment "An entry that has been withdrawn from use.  Corresponds to ISO 19135:2005 'retired'"@en ;
  skos:altlabel "withdrawn"@en ;
  skos:broader :statusDeprecated ;
  skos:definition "An entry that has been withdrawn from use.  Corresponds to ISO 19135:2005 'retired'"@en ;
  skos:exactMatch reg:statusRetired ;
  skos:prefLabel "retired"@en ;
.
:statusStable
  a :Status ;
  a owl:NamedIndividual ;
  rdfs:comment "An entry that is seen as having a reasonable measure of stability, may be used to mark the full adoption of a previously 'experimental' entry."@en ;
  skos:broader :statusValid ;
  skos:definition "An entry that is seen as having a reasonable measure of stability, may be used to mark the full adoption of a previously 'experimental' entry."@en ;
  skos:exactMatch reg:statusStable ;
  skos:inScheme :StatusScheme ;
  skos:prefLabel "stable"@en ;
.
:statusSubmitted
  a :Status ;
  a owl:NamedIndividual ;
  rdfs:comment "A proposed entry which is not yet approved for use for use. Corresponds to ISO 19135:(redraft) 'submitted'"@en ;
  skos:broader :statusNotAccepted ;
  skos:definition "A proposed entry which is not yet approved for use for use. Corresponds to ISO 19135:(redraft) 'submitted'"@en ;
  skos:exactMatch reg:statusSubmitted ;
  skos:inScheme :StatusScheme ;
  skos:prefLabel "submitted"@en ;
.
:statusSuperseded
  a :Status ;
  a owl:NamedIndividual ;
  rdfs:comment "An entry that has been replaced by a new alternative which should be used instead.  Corresponds to ISO 19135:2005 'superseded'."@en ;
  skos:altlabel "replaced"@en ;
  skos:broader :statusDeprecated ;
  skos:definition "An entry that has been replaced by a new alternative which should be used instead.  Corresponds to ISO 19135:2005 'superseded'."@en ;
  skos:exactMatch reg:statusSuperseded ;
  skos:inScheme :StatusScheme ;
  skos:prefLabel "superseded"@en ;
.
:statusValid
  a :Status ;
  a owl:NamedIndividual ;
  rdfs:comment "An entry that has been accepted into the register and is deemed fit for use. Corresponds to ISO 19135:2005 'valid'."@en ;
  skos:broader :statusAccepted ;
  skos:definition "An entry that has been accepted into the register and is deemed fit for use. Corresponds to ISO 19135:2005 'valid'."@en ;
  skos:exactMatch reg:statusValid ;
  skos:inScheme :StatusScheme ;
  skos:prefLabel "valid"@en ;
.
:wasNamedBy
  a owl:ObjectProperty ;
  rdfs:comment "The Agent (person, community, organization) that assigned the name to the Place"@en ;
  rdfs:domain :PlaceName ;
  rdfs:label "was named by"@en ;
  rdfs:range dcterms:Agent ;
  rdfs:subPropertyOf prov:wasAttributedTo ;
.
pt:PointOfInterest
  a :PlaceType ;
  a owl:NamedIndividual ;
  rdfs:label "Point of interest" ;
.
pt:Region
  a :PlaceType ;
  a owl:NamedIndividual ;
  rdfs:label "Region" ;
.
dcterms:Agent
  a owl:Class ;
.
dcterms:contributor
  a owl:ObjectProperty ;
.
dcterms:created
  a owl:DatatypeProperty ;
.
dcterms:creator
  a owl:ObjectProperty ;
.
dcterms:format
  a owl:AnnotationProperty ;
.
dcterms:identifier
  a owl:AnnotationProperty ;
  a owl:DatatypeProperty ;
.
dcterms:modified
  a owl:DatatypeProperty ;
.
dcterms:publisher
  a owl:ObjectProperty ;
.
dcterms:rights
  a owl:AnnotationProperty ;
.
dcterms:type
  a owl:ObjectProperty ;
.
reg:statusAccepted
  a owl:NamedIndividual ;
.
reg:statusDeprecated
  a owl:NamedIndividual ;
.
reg:statusExperimental
  a owl:NamedIndividual ;
.
reg:statusInvalid
  a owl:NamedIndividual ;
.
reg:statusNotAccepted
  a owl:NamedIndividual ;
.
reg:statusReserved
  a owl:NamedIndividual ;
.
reg:statusRetired
  a owl:NamedIndividual ;
.
reg:statusStable
  a owl:NamedIndividual ;
.
reg:statusSubmitted
  a owl:NamedIndividual ;
.
reg:statusSuperseded
  a owl:NamedIndividual ;
.
reg:statusValid
  a owl:NamedIndividual ;
.
<http://www.opengis.net/doc/IS/geosparql/1.0>
  a owl:NamedIndividual ;
.
rdf:Bag
  a owl:Class ;
.
rdfs:member
  a owl:ObjectProperty ;
.
skos:altlabel
  a owl:AnnotationProperty ;
.
skos:broader
  a owl:ObjectProperty ;
.
skos:exactMatch
  a owl:ObjectProperty ;
.
skos:inScheme
  a owl:ObjectProperty ;
.
skos:topConceptOf
  a owl:ObjectProperty ;
.
prof:hasArtifact
  a owl:ObjectProperty ;
.
prof:hasResource
  a owl:ObjectProperty ;
.
prof:hasRole
  a owl:ObjectProperty ;
.
prof:isProfileOf
  a owl:ObjectProperty ;
.
<http://www.w3.org/ns/dx/prof/role/schema>
  a owl:NamedIndividual ;
.
<http://www.w3.org/ns/dx/prof/role/specification>
  a owl:NamedIndividual ;
.
prov:wasAttributedTo
  a owl:ObjectProperty ;
.
<https://orcid.org/0000-0002-3884-3420>
  a owl:NamedIndividual ;
  a schema:Person ;
  schema:affiliation [
      schema:identifier "http://catalogue.linked.data.gov.au/org/csiro"^^xsd:anyURI ;
      schema:name "CSIRO" ;
    ] ;
  schema:email <mailto:simon.cox@csiro.au> ;
  schema:identifier "https://orcid.org/0000-0002-3884-3420"^^xsd:anyURI ;
  schema:name "Simon J D Cox"@en ;
.
<https://orcid.org/0000-0002-4643-7289>
  a owl:NamedIndividual ;
  a schema:Person ;
  schema:affiliation [
      schema:identifier "http://catalogue.linked.data.gov.au/org/ga"^^xsd:anyURI ;
      schema:name "Geoscience Australia" ;
    ] ;
  schema:email <mailto:irina.bastrakova@ga.gov.au> ;
  schema:identifier "https://orcid.org/0000-0002-4643-7289"^^xsd:anyURI ;
  schema:name "Irina Bastrakova"@en ;
.
<https://orcid.org/0000-0002-8742-7730>
  a owl:NamedIndividual ;
  a schema:Person ;
  schema:affiliation [
      schema:name "Surround Australia" ;
      schema:uri <https://surroundaustralia.com/> ;
    ] ;
  schema:email <mailto:nicholas.car@surroundaustralia.com> ;
  schema:identifier "https://orcid.org/0000-0002-8742-7730"^^xsd:anyURI ;
  schema:name "Nicholas Car"@en ;
.
<https://orcid.org/0000-0003-3425-0780>
  a owl:NamedIndividual ;
  a schema:Person ;
  schema:affiliation [
      schema:identifier "http://catalogue.linked.data.gov.au/org/anu"^^xsd:anyURI ;
      schema:name "Australian National University" ;
    ] ;
  schema:affiliation [
      schema:identifier "http://catalogue.linked.data.gov.au/org/anu"^^xsd:anyURI ;
      schema:name "Australian National University" ;
    ] ;
  schema:email <mailto:armin.haller@anu.edu.au> ;
  schema:identifier "https://orcid.org/0000-0003-3425-0780"^^xsd:anyURI ;
  schema:name "Armin Haller"@en ;
.
schema:Person
  a owl:Class ;
.
schema:affiliation
  a owl:AnnotationProperty ;
.
schema:email
  a owl:AnnotationProperty ;
.
schema:identifier
  a owl:AnnotationProperty ;
.
schema:memberOf
  a owl:AnnotationProperty ;
.
schema:name
  a owl:AnnotationProperty ;
.
schema:uri
  a owl:AnnotationProperty ;
.
[
  dcterms:format <https://w3id.org/mediatype/text/html> ;
  prof:hasArtifact <http://linked.data.gov.au/def/placenames> ;
  prof:hasRole <http://www.w3.org/ns/dx/prof/role/specification> ;
].
[
  dcterms:format <https://w3id.org/mediatype/text/turtle> ;
  prof:hasArtifact <http://linked.data.gov.au/def/placenames.ttl> ;
  prof:hasRole <http://www.w3.org/ns/dx/prof/role/schema> ;
].
